Fixed transcTheory for temp_loose_equality

src/real/transcScript.sml
@@ -2,20 +2,23 @@
 (* Definitions of the transcendental functions etc.                          *)
 (*===========================================================================*)
 
-(*
-app load ["hol88Lib",
-          "numLib",
-          "reduceLib",
-          "pairTheory",
-          "jrhUtils",
-          "powserTheory",
-          "Diff",
-          "mesonLib",
-          "RealArith"];
+(* ----------------------------------------------------------------------
+    Exponentiation with real exponents (rpow)
 
-*)
+    Contributed by
 
-open HolKernel Parse boolLib;
+       Umair Siddique
+
+       Email: umair.siddique@rcms.nust.edu.pk
+       DATE: 29-12-2010
+
+       System Analysis & Verification (sAvE)  LAB
+
+       National University of Sciences and Technology (NUST)
+       Ialamabad,Pakistan
+    ---------------------------------------------------------------------- *)
+
+open HolKernel Parse bossLib boolLib;
 
 open hol88Lib
      reduceLib
@@ -23,7 +26,7 @@ open hol88Lib
      numTheory
      prim_recTheory
      arithmeticTheory
-     realTheory
+     realTheory realSimps
      metricTheory
      netsTheory
      seqTheory
@@ -37,9 +40,6 @@ open hol88Lib
      RealArith;
 
 val _ = new_theory "transc";
-val _ = ParseExtras.temp_loose_equality()
-
-
 val _ = Parse.reveal "B";
 
 (*---------------------------------------------------------------------------*)
@@ -442,7 +442,7 @@ val EXP_MONO_IMP = store_thm("EXP_MONO_IMP",
   REPEAT GEN_TAC THEN DISCH_THEN(MP_TAC o
     MATCH_MP EXP_LT_1 o ONCE_REWRITE_RULE[GSYM REAL_SUB_LT]) THEN
   REWRITE_TAC[EXP_SUB] THEN
-  SUBGOAL_THEN “&1 < exp(y) / exp(x) =
+  SUBGOAL_THEN “&1 < exp(y) / exp(x) <=>
                  (&1 * exp(x)) < ((exp(y) / exp(x)) * exp(x))” SUBST1_TAC THENL
    [CONV_TAC SYM_CONV THEN MATCH_MP_TAC REAL_LT_RMUL THEN
     MATCH_ACCEPT_TAC EXP_POS_LT,
@@ -450,7 +450,7 @@ val EXP_MONO_IMP = store_thm("EXP_MONO_IMP",
     REWRITE_TAC[REAL_MUL_LID, REAL_MUL_RID]]);
 
 val EXP_MONO_LT = store_thm("EXP_MONO_LT",
-  “!x y. exp(x) < exp(y) = x < y”,
+  “!x y. exp(x) < exp(y) <=> x < y”,
   REPEAT GEN_TAC THEN EQ_TAC THENL
    [CONV_TAC CONTRAPOS_CONV THEN REWRITE_TAC[REAL_NOT_LT] THEN
     REWRITE_TAC[REAL_LE_LT] THEN
@@ -460,12 +460,12 @@ val EXP_MONO_LT = store_thm("EXP_MONO_LT",
     MATCH_ACCEPT_TAC EXP_MONO_IMP]);
 
 val EXP_MONO_LE = store_thm("EXP_MONO_LE",
-  “!x y. exp(x) <= exp(y) = x <= y”,
+  “!x y. exp(x) <= exp(y) <=> x <= y”,
   REPEAT GEN_TAC THEN REWRITE_TAC[GSYM REAL_NOT_LT] THEN
   REWRITE_TAC[EXP_MONO_LT]);
 
 val EXP_INJ = store_thm("EXP_INJ",
-  “!x y. (exp(x) = exp(y)) = (x = y)”,
+  “!x y. (exp(x) = exp(y)) <=> (x = y)”,
   REPEAT GEN_TAC THEN ONCE_REWRITE_TAC[GSYM REAL_LE_ANTISYM] THEN
   REWRITE_TAC[EXP_MONO_LE]);
 
@@ -557,7 +557,7 @@ val LN_EXP = store_thm("LN_EXP",
   EXISTS_TAC “x:real” THEN REFL_TAC);
 
 val EXP_LN = store_thm("EXP_LN",
-  “!x. (exp(ln x) = x) = &0 < x”,
+  “!x. (exp(ln x) = x) <=> &0 < x”,
   GEN_TAC THEN EQ_TAC THENL
    [DISCH_THEN(SUBST1_TAC o SYM) THEN MATCH_ACCEPT_TAC EXP_POS_LT,
     DISCH_THEN(X_CHOOSE_THEN “y:real” MP_TAC o MATCH_MP EXP_TOTAL) THEN
@@ -604,14 +604,14 @@ val LN_DIV = store_thm("LN_DIV",
     REWRITE_TAC[real_sub]]);
 
 val LN_MONO_LT = store_thm("LN_MONO_LT",
-  “!x y. &0 < x /\ &0 < y ==> (ln(x) < ln(y) = x < y)”,
+  “!x y. &0 < x /\ &0 < y ==> (ln(x) < ln(y) <=> x < y)”,
   REPEAT GEN_TAC THEN STRIP_TAC THEN
   EVERY_ASSUM(fn th => GEN_REWR_TAC (RAND_CONV o ONCE_DEPTH_CONV)
     [SYM(REWRITE_RULE[GSYM EXP_LN] th)]) THEN
   CONV_TAC SYM_CONV THEN MATCH_ACCEPT_TAC EXP_MONO_LT);
 
 val LN_MONO_LE = store_thm("LN_MONO_LE",
-  “!x y. &0 < x /\ &0 < y ==> (ln(x) <= ln(y) = x <= y)”,
+  “!x y. &0 < x /\ &0 < y ==> (ln(x) <= ln(y) <=> x <= y)”,
   REPEAT GEN_TAC THEN STRIP_TAC THEN
   EVERY_ASSUM(fn th => GEN_REWR_TAC (RAND_CONV o ONCE_DEPTH_CONV)
     [SYM(REWRITE_RULE[GSYM EXP_LN] th)]) THEN
@@ -782,27 +782,31 @@ val ROOT_POS = store_thm("ROOT_POS",
     POP_ASSUM ACCEPT_TAC,
     POP_ASSUM(SUBST1_TAC o SYM) THEN REWRITE_TAC[ROOT_0, REAL_LE_REFL]]);
 
-val ROOT_POS_UNIQ = store_thm("ROOT_POS_UNIQ",
- Term`!n x y. &0 <= x /\ &0 <= y /\ (y pow (SUC n) = x)
-           ==> (root (SUC n) x = y)`,
+Theorem ROOT_POS_UNIQ :
+   !n x y. &0 <= x /\ &0 <= y /\ (y pow (SUC n) = x)
+           ==> (root (SUC n) x = y)
+Proof
   REPEAT GEN_TAC THEN DISCH_THEN(CONJUNCTS_THEN2 ASSUME_TAC MP_TAC) THEN
   DISCH_THEN(CONJUNCTS_THEN2 MP_TAC (SUBST1_TAC o SYM)) THEN
-  REWRITE_TAC[POW_ROOT_POS]);;
+  REWRITE_TAC[POW_ROOT_POS]
+QED
 
-val ROOT_MUL = store_thm("ROOT_MUL",
- Term`!n x y. &0 <= x /\ &0 <= y
-           ==> (root(SUC n) (x * y) = root(SUC n) x * root(SUC n) y)`,
+Theorem ROOT_MUL :
+   !n x y. &0 <= x /\ &0 <= y
+           ==> (root(SUC n) (x * y) = root(SUC n) x * root(SUC n) y)
+Proof
   REPEAT STRIP_TAC THEN MATCH_MP_TAC ROOT_POS_UNIQ THEN
   REWRITE_TAC [POW_MUL] THEN REPEAT CONJ_TAC THENL
   [MATCH_MP_TAC REAL_LE_MUL THEN ASM_REWRITE_TAC[],
    MATCH_MP_TAC REAL_LE_MUL THEN CONJ_TAC THEN MATCH_MP_TAC ROOT_POS
    THEN ASM_REWRITE_TAC[],
-   IMP_RES_TAC ROOT_POW_POS THEN ASM_REWRITE_TAC[]]);
+   IMP_RES_TAC ROOT_POW_POS THEN ASM_REWRITE_TAC[]]
+QED
 
-
-val ROOT_INV = store_thm("ROOT_INV",
- Term`!n x. &0 <= x ==> (root(SUC n) (inv x) = inv(root(SUC n) x))`,
-REPEAT STRIP_TAC THEN MATCH_MP_TAC ROOT_POS_UNIQ THEN REPEAT CONJ_TAC THENL
+Theorem ROOT_INV :
+   !n x. &0 <= x ==> (root(SUC n) (inv x) = inv(root(SUC n) x))
+Proof
+ REPEAT STRIP_TAC THEN MATCH_MP_TAC ROOT_POS_UNIQ THEN REPEAT CONJ_TAC THENL
  [IMP_RES_THEN ACCEPT_TAC REAL_LE_INV,
   MATCH_MP_TAC REAL_LE_INV THEN IMP_RES_THEN (TRY o MATCH_ACCEPT_TAC) ROOT_POS,
   IMP_RES_TAC ROOT_POW_POS THEN MP_TAC (SPEC_ALL ROOT_POS)
@@ -812,20 +816,24 @@ REPEAT STRIP_TAC THEN MATCH_MP_TAC ROOT_POS_UNIQ THEN REPEAT CONJ_TAC THENL
        REWRITE_TAC [GSYM th]) POW_INV THEN ASM_REWRITE_TAC[],
      POP_ASSUM (ASSUME_TAC o SYM) THEN ASM_REWRITE_TAC[] THEN
      PAT_X_ASSUM (Term `$! M`) (SUBST1_TAC o SYM o SPEC_ALL)
-      THEN ASM_REWRITE_TAC[REAL_INV_0,POW_0]]])
+      THEN ASM_REWRITE_TAC[REAL_INV_0,POW_0]]]
+QED
 
-val ROOT_DIV = store_thm("ROOT_DIV",
- Term`!n x y. &0 <= x /\ &0 <= y
-           ==> (root(SUC n) (x / y) = root(SUC n) x / root(SUC n) y)`,
-REWRITE_TAC [real_div] THEN REPEAT STRIP_TAC THEN IMP_RES_TAC REAL_LE_INV
+Theorem ROOT_DIV :
+   !n x y. &0 <= x /\ &0 <= y
+           ==> (root(SUC n) (x / y) = root(SUC n) x / root(SUC n) y)
+Proof
+ REWRITE_TAC [real_div] THEN REPEAT STRIP_TAC THEN IMP_RES_TAC REAL_LE_INV
  THEN MP_TAC (SPECL [Term`n:num`, Term`x:real`, Term`inv y`] ROOT_MUL)
  THEN ASM_REWRITE_TAC[] THEN STRIP_TAC THEN ASM_REWRITE_TAC[]
  THEN IMP_RES_TAC (SPECL [Term`n:num`, Term`y:real`] ROOT_INV)
- THEN ASM_REWRITE_TAC[]);
+ THEN ASM_REWRITE_TAC[]
+QED
 
-
-val ROOT_MONO_LE = store_thm("ROOT_MONO_LE",
- Term`!x y. &0 <= x /\ x <= y ==> root(SUC n) x <= root(SUC n) y`,
+(* added ‘n’ into quantifiers *)
+Theorem ROOT_MONO_LE :
+   !n x y. &0 <= x /\ x <= y ==> root(SUC n) x <= root(SUC n) y
+Proof
   REPEAT STRIP_TAC THEN SUBGOAL_THEN (Term`&0 <= y`) ASSUME_TAC THENL
    [ASM_MESON_TAC[REAL_LE_TRANS], ALL_TAC] THEN
   UNDISCH_TAC (Term`x <= y`) THEN CONV_TAC CONTRAPOS_CONV THEN
@@ -835,7 +843,8 @@ val ROOT_MONO_LE = store_thm("ROOT_MONO_LE",
    (CONJUNCTS_THEN SUBST1_TAC)
   THENL [IMP_RES_TAC (GSYM ROOT_POW_POS) THEN ASM_MESON_TAC[], ALL_TAC] THEN
   MATCH_MP_TAC REAL_POW_LT2 THEN
-  ASM_REWRITE_TAC[NOT_SUC] THEN MATCH_MP_TAC ROOT_POS THEN ASM_REWRITE_TAC[]);
+  ASM_REWRITE_TAC[NOT_SUC] THEN MATCH_MP_TAC ROOT_POS THEN ASM_REWRITE_TAC[]
+QED
 
 val SQRT_0 = store_thm("SQRT_0",
   “sqrt(&0) = &0”,
@@ -846,77 +855,78 @@ val SQRT_1 = store_thm("SQRT_1",
   REWRITE_TAC[sqrt, TWO, ROOT_1]);
 
 val SQRT_POS_LT = store_thm("SQRT_POS_LT",
- Term`!x. &0 < x ==> &0 < sqrt(x)`,
+  “!x. &0 < x ==> &0 < sqrt(x)”,
  REWRITE_TAC [sqrt,TWO] THEN REPEAT STRIP_TAC
   THEN IMP_RES_TAC ROOT_LN THEN ASM_REWRITE_TAC[EXP_POS_LT]);
 
 val SQRT_POS_LE = store_thm("SQRT_POS_LE",
- Term`!x. &0 <= x ==> &0 <= sqrt(x)`,
-  REWRITE_TAC[REAL_LE_LT] THEN MESON_TAC[SQRT_POS_LT, SQRT_0]);;
+  “!x. &0 <= x ==> &0 <= sqrt(x)”,
+  REWRITE_TAC[REAL_LE_LT] THEN MESON_TAC[SQRT_POS_LT, SQRT_0]);
 
 val SQRT_POW2 = store_thm("SQRT_POW2",
-  “!x. (sqrt(x) pow 2 = x) = &0 <= x”,
+  “!x. (sqrt(x) pow 2 = x) <=> &0 <= x”,
   GEN_TAC THEN EQ_TAC THENL
    [DISCH_THEN(SUBST1_TAC o SYM) THEN MATCH_ACCEPT_TAC REAL_LE_POW2,
     REWRITE_TAC[sqrt, TWO, ROOT_POW_POS]]);
 
 val SQRT_POW_2 = store_thm("SQRT_POW_2",
- Term `!x. &0 <= x ==> (sqrt(x) pow 2 = x)`,
-  REWRITE_TAC[SQRT_POW2]);;
+  “!x. &0 <= x ==> (sqrt(x) pow 2 = x)”,
+  REWRITE_TAC[SQRT_POW2]);
 
 val POW_2_SQRT = store_thm("POW_2_SQRT",
- Term`&0 <= x ==> (sqrt(x pow 2) = x)`,
+  “&0 <= x ==> (sqrt(x pow 2) = x)”,
  REWRITE_TAC [sqrt,TWO,POW_ROOT_POS]);
 
 val SQRT_POS_UNIQ = store_thm("SQRT_POS_UNIQ",
- Term`!x y. &0 <= x /\ &0 <= y /\ (y pow 2 = x)
-           ==> (sqrt x = y)`,
+  “!x y. &0 <= x /\ &0 <= y /\ (y pow 2 = x) ==> (sqrt x = y)”,
   REWRITE_TAC[sqrt, TWO, ROOT_POS_UNIQ]);
 
 val SQRT_MUL = store_thm("SQRT_MUL",
- Term`!x y. &0 <= x /\ &0 <= y
-           ==> (sqrt(x * y) = sqrt x * sqrt y)`,
-  REWRITE_TAC[sqrt, TWO, ROOT_MUL]);;
+  “!x y. &0 <= x /\ &0 <= y ==> (sqrt(x * y) = sqrt x * sqrt y)”,
+  REWRITE_TAC[sqrt, TWO, ROOT_MUL]);
 
 val SQRT_INV = store_thm("SQRT_INV",
- Term`!x. &0 <= x ==> (sqrt (inv x) = inv(sqrt x))`,
-  REWRITE_TAC[sqrt, TWO, ROOT_INV]);;
+  “!x. &0 <= x ==> (sqrt (inv x) = inv(sqrt x))”,
+  REWRITE_TAC[sqrt, TWO, ROOT_INV]);
 
 val SQRT_DIV = store_thm("SQRT_DIV",
- Term`!x y. &0 <= x /\ &0 <= y
-           ==> (sqrt (x / y) = sqrt x / sqrt y)`,
-  REWRITE_TAC[sqrt, TWO, ROOT_DIV]);;
+  “!x y. &0 <= x /\ &0 <= y ==> (sqrt (x / y) = sqrt x / sqrt y)”,
+  REWRITE_TAC[sqrt, TWO, ROOT_DIV]);
 
 val SQRT_MONO_LE = store_thm("SQRT_MONO_LE",
- Term`!x y. &0 <= x /\ x <= y ==> sqrt(x) <= sqrt(y)`,
-  REWRITE_TAC[sqrt, TWO, ROOT_MONO_LE]);;
+  “!x y. &0 <= x /\ x <= y ==> sqrt(x) <= sqrt(y)”,
+  REWRITE_TAC[sqrt, TWO, ROOT_MONO_LE]);
 
 val lem = prove(Term`0<2:num`, REWRITE_TAC[TWO,LESS_0]);
 
-val EVEN_MOD = prove
- (Term `!n. EVEN(n) = (n MOD 2 = 0)`,
+Theorem EVEN_MOD[local] :
+    !n. EVEN(n) = (n MOD 2 = 0)
+Proof
   GEN_TAC THEN REWRITE_TAC[EVEN_EXISTS] THEN ONCE_REWRITE_TAC[MULT_SYM] THEN
   EQ_TAC THEN STRIP_TAC THENL
   [ASM_REWRITE_TAC [MP (SPEC (Term`2:num`) MOD_EQ_0) lem],
    EXISTS_TAC (Term `n DIV 2`) THEN
      MP_TAC (CONJUNCT1 (SPEC (Term `n:num`) (MATCH_MP DIVISION lem))) THEN
-     ASM_REWRITE_TAC [ADD_CLAUSES]]);
+     ASM_REWRITE_TAC [ADD_CLAUSES]]
+QED
 
-val SQRT_EVEN_POW2 = store_thm("SQRT_EVEN_POW2",
- Term`!n. EVEN n ==> (sqrt(&2 pow n) = &2 pow (n DIV 2))`,
- GEN_TAC THEN REWRITE_TAC[EVEN_MOD] THEN DISCH_TAC THEN
+Theorem SQRT_EVEN_POW2 :
+    !n. EVEN n ==> (sqrt(&2 pow n) = &2 pow (n DIV 2))
+Proof
+  GEN_TAC THEN REWRITE_TAC[EVEN_MOD] THEN DISCH_TAC THEN
   MATCH_MP_TAC SQRT_POS_UNIQ THEN REPEAT CONJ_TAC THENL
   [MATCH_MP_TAC POW_POS THEN REWRITE_TAC [REAL_POS],
    MATCH_MP_TAC POW_POS THEN REWRITE_TAC [REAL_POS],
    REWRITE_TAC [REAL_POW_POW] THEN AP_TERM_TAC THEN
    MP_TAC (CONJUNCT1 (SPEC (Term `n:num`) (MATCH_MP DIVISION lem)))
    THEN ASM_REWRITE_TAC [ADD_CLAUSES] THEN DISCH_THEN (SUBST1_TAC o SYM)
-   THEN REFL_TAC]);
+   THEN REFL_TAC]
+QED
 
-
-val REAL_DIV_SQRT = store_thm("REAL_DIV_SQRT",
- Term`!x. &0 <= x ==> (x / sqrt(x) = sqrt(x))`,
- GEN_TAC THEN ASM_CASES_TAC (Term`x = &0`) THENL
+Theorem REAL_DIV_SQRT :
+    !x. &0 <= x ==> (x / sqrt(x) = sqrt(x))
+Proof
+  GEN_TAC THEN ASM_CASES_TAC (Term`x = &0`) THENL
    [ASM_REWRITE_TAC[SQRT_0, real_div, REAL_MUL_LZERO], ALL_TAC] THEN
   DISCH_TAC THEN CONV_TAC SYM_CONV THEN MATCH_MP_TAC SQRT_POS_UNIQ THEN
   ASM_REWRITE_TAC[] THEN IMP_RES_TAC SQRT_POS_LE THEN
@@ -935,7 +945,8 @@ val REAL_DIV_SQRT = store_thm("REAL_DIV_SQRT",
      PAT_X_ASSUM (Term `& 0 = _`) (SUBST_ALL_TAC o SYM) THEN
      IMP_RES_TAC REAL_LT_REFL,
    PAT_X_ASSUM (Term `& 0 = _`) (SUBST_ALL_TAC o SYM)
-   THEN REWRITE_TAC [POW_0, TWO, REAL_MUL_LZERO]]]);
+   THEN REWRITE_TAC [POW_0, TWO, REAL_MUL_LZERO]]]
+QED
 
 val SQRT_EQ = store_thm("SQRT_EQ",
   “!x y. (x pow 2 = y) /\ (&0 <= x) ==> (x = (sqrt(y)))”,
@@ -1316,7 +1327,7 @@ val COS_ISZERO = store_thm("COS_ISZERO",
       REWRITE_TAC[DIFF_COS]],
     ASM_REWRITE_TAC[] THEN BETA_TAC THEN
     MAP_EVERY X_GEN_TAC [“x1:real”, “x2:real”] THEN
-    GEN_REWR_TAC I  [TAUT_CONV “a:bool = ~~a”] THEN
+    GEN_REWR_TAC I  [TAUT_CONV “a:bool <=> ~~a”] THEN
     PURE_REWRITE_TAC[NOT_IMP] THEN REWRITE_TAC[] THEN STRIP_TAC THEN
     MP_TAC(SPECL [“x1:real”, “x2:real”] REAL_LT_TOTAL) THEN
     SUBGOAL_THEN “(!x. cos differentiable x) /\ (!x. cos contl x)”
@@ -1596,7 +1607,7 @@ val SIN_TOTAL = store_thm("SIN_TOTAL",
         ?!x.  ~(pi / &2) <= x /\ x <= pi / &2 /\ (sin(x) = y)”,
   GEN_TAC THEN DISCH_TAC THEN
   SUBGOAL_THEN “!x. ~(pi / &2) <= x /\ x <= pi / &2 /\ (sin(x) = y)
-                           =
+                           <=>
                        &0 <= (x + pi / &2) /\
                        (x + pi / &2) <= pi  /\
                        (cos(x + pi / &2) = ~y)”
@@ -1682,8 +1693,8 @@ val SIN_ZERO_LEMMA = store_thm("SIN_ZERO_LEMMA",
   REWRITE_TAC[ONCE_REWRITE_RULE[REAL_ADD_SYM] REAL_ADD_SUB]);
 
 val COS_ZERO = store_thm("COS_ZERO",
-  “!x. (cos(x) = &0) = (?n. ~EVEN n /\ (x = &n * (pi / &2))) \/
-                       (?n. ~EVEN n /\ (x = ~(&n * (pi / &2))))”,
+  “!x. (cos(x) = &0) <=> (?n. ~EVEN n /\ (x = &n * (pi / &2))) \/
+                         (?n. ~EVEN n /\ (x = ~(&n * (pi / &2))))”,
   GEN_TAC THEN EQ_TAC THENL
    [DISCH_TAC THEN DISJ_CASES_TAC (SPECL [“&0”, “x:real”] REAL_LE_TOTAL) THENL
      [DISJ1_TAC THEN MATCH_MP_TAC COS_ZERO_LEMMA THEN ASM_REWRITE_TAC[],
@@ -1703,8 +1714,8 @@ val COS_ZERO = store_thm("COS_ZERO",
     REWRITE_TAC[REAL_SUB_RZERO]]);
 
 val SIN_ZERO = store_thm("SIN_ZERO",
-  “!x. (sin(x) = &0) = (?n. EVEN n /\ (x = &n * (pi / &2))) \/
-                       (?n. EVEN n /\ (x = ~(&n * (pi / &2))))”,
+  “!x. (sin(x) = &0) <=> (?n. EVEN n /\ (x = &n * (pi / &2))) \/
+                         (?n. EVEN n /\ (x = ~(&n * (pi / &2))))”,
   GEN_TAC THEN EQ_TAC THENL
    [DISCH_TAC THEN DISJ_CASES_TAC (SPECL [“&0”, “x:real”] REAL_LE_TOTAL) THENL
      [DISJ1_TAC THEN MATCH_MP_TAC SIN_ZERO_LEMMA THEN ASM_REWRITE_TAC[],
@@ -1845,7 +1856,7 @@ val TAN_TOTAL_LEMMA = store_thm("TAN_TOTAL_LEMMA",
     REWRITE_TAC[GSYM REAL_NOT_LE, real_sub, REAL_LE_ADDR, REAL_NEG_GE0] THEN
     ASM_REWRITE_TAC[REAL_NOT_LE], ALL_TAC] THEN
   DISCH_THEN(fn th => ASSUME_TAC th THEN MP_TAC(MATCH_MP REAL_POS_NZ th)) THEN
-  REWRITE_TAC[ABS_NZ, TAUT_CONV “a ==> b ==> c = a /\ b ==> c”] THEN
+  REWRITE_TAC[ABS_NZ, TAUT_CONV “a ==> b ==> c <=> a /\ b ==> c”] THEN
   DISCH_THEN(MP_TAC o MATCH_MP REAL_LT_INV) THEN REWRITE_TAC[tan] THEN
   MATCH_MP_TAC (TAUT_CONV “(a = b) ==> a ==> b”) THEN BINOP_TAC THENL
    [MATCH_MP_TAC REAL_INVINV THEN MATCH_MP_TAC REAL_POS_NZ THEN
@@ -2246,51 +2257,58 @@ let LESS_SUC_EQ = prove(
 (* Divisions and tagged divisions etc.                                      *)
 (* ------------------------------------------------------------------------ *)
 
-val division = new_definition("division",
-Term`division(a,b) D =
+Definition division :
+   division(a,b) D <=>
      (D 0 = a) /\
      (?N. (!n. n < N ==> D(n) < D(SUC n)) /\
-          (!n. n >= N ==> (D(n) = b)))`);
+          (!n. n >= N ==> (D(n) = b)))
+End
 
-val dsize = new_definition("dsize",
- Term`dsize D =
+Definition dsize :
+   dsize D =
       @N. (!n. n < N ==> D(n) < D(SUC n)) /\
-          (!n. n >= N ==> (D(n) = D(N)))`);
+          (!n. n >= N ==> (D(n) = D(N)))
+End
 
-val tdiv = new_definition("tdiv",
- Term`tdiv(a,b) (D,p) =
+Definition tdiv :
+   tdiv(a,b) (D,p) <=>
      division(a,b) D /\
-     (!n. D(n) <= p(n) /\ p(n) <= D(SUC n))`);
+     (!n. D(n) <= p(n) /\ p(n) <= D(SUC n))
+End
 
 (* ------------------------------------------------------------------------ *)
 (* Gauges and gauge-fine divisions                                          *)
 (* ------------------------------------------------------------------------ *)
 
-val gauge = new_definition("gauge",
-  Term`gauge(E) (g:real->real) = !x. E x ==> &0 < g(x)`);;
+Definition gauge :
+   gauge(E) (g:real->real) = !x. E x ==> &0 < g(x)
+End
 
-val fine = new_definition("fine",
- Term`fine(g:real->real) (D,p) =
-     !n. n < dsize D ==> D(SUC n) - D(n) < g(p(n))`);
+Definition fine :
+   fine(g:real->real) (D,p) =
+     !n. n < dsize D ==> D(SUC n) - D(n) < g(p(n))
+End
 
 (* ------------------------------------------------------------------------ *)
 (* Riemann sum                                                              *)
 (* ------------------------------------------------------------------------ *)
 
-val rsum = new_definition("rsum",
-  Term`rsum (D,(p:num->real)) f =
-        sum(0,dsize(D))(\n. f(p n) * (D(SUC n) - D(n)))`);
+Definition rsum :
+   rsum (D,(p:num->real)) f =
+        sum(0,dsize(D))(\n. f(p n) * (D(SUC n) - D(n)))
+End
 
 (* ------------------------------------------------------------------------ *)
 (* Gauge integrability (definite)                                           *)
 (* ------------------------------------------------------------------------ *)
 
-val Dint = new_definition("Dint",
- Term `Dint(a,b) f k =
-        !e. &0 < e ==>
+Definition Dint :
+   Dint(a,b) f k <=>
+       !e. &0 < e ==>
            ?g. gauge(\x. a <= x /\ x <= b) g /\
                !D p. tdiv(a,b) (D,p) /\ fine(g)(D,p) ==>
-                   abs(rsum(D,p) f - k) < e`);;
+                   abs(rsum(D,p) f - k) < e
+End
 
 (* ------------------------------------------------------------------------ *)
 (* Useful lemmas about the size of `trivial` divisions etc.                 *)
@@ -2329,12 +2347,13 @@ val DIVISION_1 = store_thm("DIVISION_1",
       THEN ASM_CASES_TAC (Term `n:num = 0`) THEN
       ASM_REWRITE_TAC[CONJUNCT1 LE, GSYM NOT_SUC, NOT_SUC]]]);
 
-val LESS_1 = prove (Term`!x:num. x < 1 = (x = 0)`,
+val LESS_1 = prove (Term`!x:num. x < 1 <=> (x = 0)`,
  INDUCT_TAC THEN
   REWRITE_TAC [ONE,LESS_0,LESS_MONO_EQ,NOT_LESS_0,GSYM SUC_NOT]);
 
-val DIVISION_SINGLE = store_thm("DIVISION_SINGLE",
-  Term `!a b. a <= b ==> division(a,b)(\n. if (n = 0) then a else b)`,
+Theorem DIVISION_SINGLE :
+    !a b. a <= b ==> division(a,b)(\n. if (n = 0) then a else b)
+Proof
   REPEAT GEN_TAC THEN DISCH_TAC THEN REWRITE_TAC[division] THEN
   BETA_TAC THEN REWRITE_TAC[] THEN
   POP_ASSUM(DISJ_CASES_TAC o REWRITE_RULE[REAL_LE_LT]) THENL
@@ -2345,20 +2364,24 @@ val DIVISION_SINGLE = store_thm("DIVISION_SINGLE",
       COND_CASES_TAC THEN ASM_REWRITE_TAC[ONE] THEN
       REWRITE_TAC[LE, NOT_SUC]],
     EXISTS_TAC (Term `0:num`) THEN REWRITE_TAC[NOT_LESS_0] THEN
-    ASM_REWRITE_TAC[COND_ID]]);
+    ASM_REWRITE_TAC[COND_ID]]
+QED
 
-val DIVISION_LHS = store_thm("DIVISION_LHS",
-  Term `!D a b. division(a,b) D ==> (D(0) = a)`,
+Theorem DIVISION_LHS :
+    !D a b. division(a,b) D ==> (D(0) = a)
+Proof
   REPEAT GEN_TAC THEN REWRITE_TAC[division] THEN
-  DISCH_THEN(fn th => REWRITE_TAC[th]));
+  DISCH_THEN(fn th => REWRITE_TAC[th])
+QED
 
-val DIVISION_THM = store_thm("DIVISION_THM",
- Term `!D a b.
+Theorem DIVISION_THM :
+    !D a b.
          division(a,b) D
-           =
+           <=>
          (D(0) = a) /\
          (!n. n < (dsize D) ==> D(n) < D(SUC n)) /\
-         (!n. n >= (dsize D) ==> (D(n) = b))`,
+         (!n. n >= (dsize D) ==> (D(n) = b))
+Proof
   REPEAT GEN_TAC THEN REWRITE_TAC[division] THEN
   EQ_TAC THEN DISCH_TAC THEN ASM_REWRITE_TAC[] THENL
    [ALL_TAC, EXISTS_TAC (Term `dsize D`) THEN ASM_REWRITE_TAC[]] THEN
@@ -2383,16 +2406,20 @@ val DIVISION_THM = store_thm("DIVISION_THM",
     MP_TAC(SPEC (Term`SUC N`) th)) THEN
     REWRITE_TAC[GREATER_EQ, LESS_EQ_SUC_REFL, LESS_EQ_REFL] THEN
     DISCH_THEN SUBST1_TAC THEN DISCH_THEN SUBST1_TAC THEN
-    REWRITE_TAC[REAL_LT_REFL]]);
+    REWRITE_TAC[REAL_LT_REFL]]
+QED
 
-val DIVISION_RHS = store_thm("DIVISION_RHS",
-  Term`!D a b. division(a,b) D ==> (D(dsize D) = b)`,
+Theorem DIVISION_RHS :
+    !D a b. division(a,b) D ==> (D(dsize D) = b)
+Proof
   REPEAT GEN_TAC THEN REWRITE_TAC[DIVISION_THM] THEN
   DISCH_THEN(MP_TAC o SPEC (Term`dsize D`) o last o CONJUNCTS) THEN
-  REWRITE_TAC[GREATER_EQ, LESS_EQ_REFL]);
+  REWRITE_TAC[GREATER_EQ, LESS_EQ_REFL]
+QED
 
-val DIVISION_LT_GEN = store_thm("DIVISION_LT_GEN",
-Term`!D a b m n. division(a,b) D /\ m < n /\ n <= (dsize D) ==> D(m) < D(n)`,
+Theorem DIVISION_LT_GEN :
+   !D a b m n. division(a,b) D /\ m < n /\ n <= (dsize D) ==> D(m) < D(n)
+Proof
   REPEAT STRIP_TAC THEN UNDISCH_TAC (Term`m:num < n`) THEN
   DISCH_THEN(X_CHOOSE_THEN (Term`d:num`) MP_TAC o MATCH_MP LESS_ADD_1) THEN
   REWRITE_TAC[GSYM ADD1] THEN DISCH_THEN SUBST_ALL_TAC THEN
@@ -2410,10 +2437,12 @@ Term`!D a b m n. division(a,b) D /\ m < n /\ n <= (dsize D) ==> D(m) < D(n)`,
       REWRITE_TAC[ADD_CLAUSES] THEN
       FIRST_ASSUM(MATCH_MP_TAC o el 2 o
         CONJUNCTS o REWRITE_RULE[DIVISION_THM]) THEN
-      ASM_REWRITE_TAC[]]]);;
+      ASM_REWRITE_TAC[]]]
+QED
 
-val DIVISION_LT = store_thm("DIVISION_LT",
-  Term`!D a b. division(a,b) D ==> !n. n < (dsize D) ==> D(0) < D(SUC n)`,
+Theorem DIVISION_LT :
+   !D a b. division(a,b) D ==> !n. n < (dsize D) ==> D(0) < D(SUC n)
+Proof
   REPEAT GEN_TAC THEN REWRITE_TAC[DIVISION_THM] THEN STRIP_TAC THEN
   INDUCT_TAC THEN DISCH_THEN(fn th => ASSUME_TAC th THEN
       FIRST_ASSUM(MP_TAC o C MATCH_MP th)) THEN
@@ -2422,10 +2451,12 @@ val DIVISION_LT = store_thm("DIVISION_LT",
   ASM_REWRITE_TAC[] THEN UNDISCH_TAC (Term`D(0:num):real = a`) THEN
   DISCH_THEN(SUBST1_TAC o SYM) THEN FIRST_ASSUM MATCH_MP_TAC THEN
   MATCH_MP_TAC LESS_TRANS THEN EXISTS_TAC (Term`SUC n`) THEN
-  ASM_REWRITE_TAC[LESS_SUC_REFL]);
+  ASM_REWRITE_TAC[LESS_SUC_REFL]
+QED
 
-val DIVISION_LE = store_thm("DIVISION_LE",
-  Term`!D a b. division(a,b) D ==> a <= b`,
+Theorem DIVISION_LE :
+   !D a b. division(a,b) D ==> a <= b
+Proof
   REPEAT GEN_TAC THEN DISCH_TAC THEN
   FIRST_ASSUM(MP_TAC o MATCH_MP DIVISION_LT) THEN
   POP_ASSUM(STRIP_ASSUME_TAC o REWRITE_RULE[DIVISION_THM]) THEN
@@ -2436,16 +2467,20 @@ val DIVISION_LE = store_thm("DIVISION_LE",
   DISCH_THEN(SUBST1_TAC o SYM) THEN
   DISCH_THEN(MP_TAC o SPEC (Term`PRE(dsize D)`)) THEN
   STRUCT_CASES_TAC(SPEC (Term`dsize D`) num_CASES) THEN
-  ASM_REWRITE_TAC[PRE, REAL_LE_REFL, LESS_SUC_REFL, REAL_LT_IMP_LE]);;
+  ASM_REWRITE_TAC[PRE, REAL_LE_REFL, LESS_SUC_REFL, REAL_LT_IMP_LE]
+QED
 
-val DIVISION_GT = store_thm("DIVISION_GT",
-  Term`!D a b. division(a,b) D ==> !n. n < (dsize D) ==> D(n) < D(dsize D)`,
+Theorem DIVISION_GT :
+   !D a b. division(a,b) D ==> !n. n < (dsize D) ==> D(n) < D(dsize D)
+Proof
   REPEAT STRIP_TAC THEN MATCH_MP_TAC DIVISION_LT_GEN THEN
   MAP_EVERY EXISTS_TAC [Term`a:real`, Term`b:real`] THEN
-  ASM_REWRITE_TAC[LESS_EQ_REFL]);;
+  ASM_REWRITE_TAC[LESS_EQ_REFL]
+QED
 
-val DIVISION_EQ = store_thm("DIVISION_EQ",
-  Term`!D a b. division(a,b) D ==> ((a = b) = (dsize D = 0))`,
+Theorem DIVISION_EQ :
+   !D a b. division(a,b) D ==> ((a = b) <=> (dsize D = 0))
+Proof
   REPEAT GEN_TAC THEN DISCH_TAC THEN
   FIRST_ASSUM(MP_TAC o MATCH_MP DIVISION_LT) THEN
   POP_ASSUM(STRIP_ASSUME_TAC o REWRITE_RULE[DIVISION_THM]) THEN
@@ -2456,10 +2491,12 @@ val DIVISION_EQ = store_thm("DIVISION_EQ",
   DISCH_THEN(SUBST1_TAC o SYM) THEN
   DISCH_THEN(MP_TAC o SPEC (Term`PRE(dsize D)`)) THEN
   STRUCT_CASES_TAC(SPEC (Term`dsize D`) num_CASES) THEN
-  ASM_REWRITE_TAC[PRE, NOT_SUC, LESS_SUC_REFL, REAL_LT_IMP_NE]);
+  ASM_REWRITE_TAC[PRE, NOT_SUC, LESS_SUC_REFL, REAL_LT_IMP_NE]
+QED
 
-val DIVISION_LBOUND = store_thm("DIVISION_LBOUND",
-  Term`!D a b. division(a,b) D ==> !r. a <= D(r)`,
+Theorem DIVISION_LBOUND :
+   !D a b. division(a,b) D ==> !r. a <= D(r)
+Proof
   REPEAT GEN_TAC THEN REWRITE_TAC[DIVISION_THM] THEN STRIP_TAC THEN
   INDUCT_TAC THEN ASM_REWRITE_TAC[REAL_LE_REFL] THEN
   DISJ_CASES_TAC(SPECL [Term`SUC r`, Term`dsize D`] LESS_CASES) THENL
@@ -2473,10 +2510,12 @@ val DIVISION_LBOUND = store_thm("DIVISION_LBOUND",
      [MATCH_MP_TAC DIVISION_LE THEN
       EXISTS_TAC (Term`D:num->real`) THEN ASM_REWRITE_TAC[DIVISION_THM],
       MATCH_MP_TAC REAL_EQ_IMP_LE THEN CONV_TAC SYM_CONV THEN
-      FIRST_ASSUM MATCH_MP_TAC THEN ASM_REWRITE_TAC[GREATER_EQ]]]);;
+      FIRST_ASSUM MATCH_MP_TAC THEN ASM_REWRITE_TAC[GREATER_EQ]]]
+QED
 
-val DIVISION_LBOUND_LT = store_thm("DIVISION_LBOUND_LT",
- Term`!D a b. division(a,b) D /\ ~(dsize D = 0) ==> !n. a < D(SUC n)`,
+Theorem DIVISION_LBOUND_LT :
+   !D a b. division(a,b) D /\ ~(dsize D = 0) ==> !n. a < D(SUC n)
+Proof
   REPEAT STRIP_TAC THEN
   FIRST_ASSUM(SUBST1_TAC o SYM o MATCH_MP DIVISION_LHS) THEN
   DISJ_CASES_TAC(SPECL [Term`dsize D`, Term`SUC n`] LESS_CASES) THENL
@@ -2488,10 +2527,12 @@ val DIVISION_LBOUND_LT = store_thm("DIVISION_LBOUND_LT",
     FIRST_ASSUM(MATCH_MP_TAC o MATCH_MP DIVISION_GT) THEN
     ASM_REWRITE_TAC[GSYM NOT_LESS_EQUAL, CONJUNCT1 LE],
     FIRST_ASSUM(MATCH_MP_TAC o MATCH_MP DIVISION_LT) THEN
-    MATCH_MP_TAC OR_LESS THEN ASM_REWRITE_TAC[]]);;
+    MATCH_MP_TAC OR_LESS THEN ASM_REWRITE_TAC[]]
+QED
 
-val DIVISION_UBOUND = store_thm("DIVISION_UBOUND",
- Term`!D a b. division(a,b) D ==> !r. D(r) <= b`,
+Theorem DIVISION_UBOUND :
+   !D a b. division(a,b) D ==> !r. D(r) <= b
+Proof
   REPEAT GEN_TAC THEN REWRITE_TAC[DIVISION_THM] THEN STRIP_TAC THEN
   GEN_TAC THEN DISJ_CASES_TAC(SPECL [Term`r:num`, Term`dsize D`] LESS_CASES)
   THENL [ALL_TAC,
@@ -2533,24 +2574,27 @@ val DIVISION_UBOUND = store_thm("DIVISION_UBOUND",
   COND_CASES_TAC THENL
    [REWRITE_TAC[SUB_EQ_0, LESS_EQ_MONO] THEN
     ASM_REWRITE_TAC[GSYM NOT_LESS],
-    DISCH_THEN (SUBST1_TAC o SYM) THEN REWRITE_TAC[SUB_MONO_EQ]]);
+    DISCH_THEN (SUBST1_TAC o SYM) THEN REWRITE_TAC[SUB_MONO_EQ]]
+QED
 
-val DIVISION_UBOUND_LT = store_thm("DIVISION_UBOUND_LT",
- Term`!D a b n. division(a,b) D /\ n < dsize D ==> D(n) < b`,
+Theorem DIVISION_UBOUND_LT :
+   !D a b n. division(a,b) D /\ n < dsize D ==> D(n) < b
+Proof
   REPEAT STRIP_TAC THEN
   FIRST_ASSUM(SUBST1_TAC o SYM o MATCH_MP DIVISION_RHS) THEN
   FIRST_ASSUM(MATCH_MP_TAC o MATCH_MP DIVISION_GT) THEN
-  ASM_REWRITE_TAC[]);
+  ASM_REWRITE_TAC[]
+QED
 
 (* ------------------------------------------------------------------------ *)
 (* Divisions of adjacent intervals can be combined into one                 *)
 (* ------------------------------------------------------------------------ *)
 
-val D_tm = Term`\n. if n < dsize D1 then D1(n) else D2(n - dsize D1)`
-and p_tm = Term`\n. if n < dsize D1 then (p1:num->real)(n) else p2(n - dsize D1)`;
+val D_tm = “\n. if n < dsize D1 then D1(n) else D2(n - dsize D1)”;
+val p_tm = “\n. if n < dsize D1 then (p1:num->real)(n) else p2(n - dsize D1)”;
 
-val DIVISION_APPEND_LEMMA1 = prove(
- Term `!a b c D1 D2.
+Theorem DIVISION_APPEND_LEMMA1[local] :
+  !a b c D1 D2.
    division(a,b) D1 /\ division(b,c) D2
     ==>
     (!n. n < dsize D1 + dsize D2
@@ -2562,7 +2606,8 @@ val DIVISION_APPEND_LEMMA1 = prove(
          ==>
          ((\n. if n<dsize D1 then D1(n) else D2(n - dsize D1)) (n)
            =
-          (\n. if n<dsize D1 then D1(n) else D2(n - dsize D1)) (dsize D1 + dsize D2)))`,
+          (\n. if n<dsize D1 then D1(n) else D2(n - dsize D1)) (dsize D1 + dsize D2)))
+Proof
   REPEAT GEN_TAC THEN STRIP_TAC THEN CONJ_TAC THEN
   X_GEN_TAC (Term`n:num`) THEN DISCH_TAC THEN BETA_TAC THENL
    [ASM_CASES_TAC (Term`SUC n < dsize D1`) THEN ASM_REWRITE_TAC[] THENL
@@ -2606,15 +2651,17 @@ val DIVISION_APPEND_LEMMA1 = prove(
        (SUBST1_TAC o MATCH_MP DIVISION_RHS)) THEN
       FIRST_ASSUM(MATCH_MP_TAC o el 3 o CONJUNCTS o
         REWRITE_RULE[DIVISION_THM]) THEN
-      REWRITE_TAC[GREATER_EQ, LESS_EQ_ADD]]]);
+      REWRITE_TAC[GREATER_EQ, LESS_EQ_ADD]]]
+QED
 
-val DIVISION_APPEND_LEMMA2 = prove(
- Term`!a b c D1 D2.
+Theorem DIVISION_APPEND_LEMMA2[local] :
+   !a b c D1 D2.
     division(a,b) D1 /\ division(b,c) D2
       ==>
       (dsize(\n. if n < dsize D1 then D1(n) else D2(n - dsize D1))
          =
-       dsize D1 + dsize D2)`,
+       dsize D1 + dsize D2)
+Proof
   REPEAT STRIP_TAC THEN GEN_REWRITE_TAC LAND_CONV [] [dsize] THEN
   MATCH_MP_TAC SELECT_UNIQUE THEN
   X_GEN_TAC (Term`N:num`) THEN BETA_TAC THEN EQ_TAC THENL
@@ -2707,13 +2754,16 @@ val DIVISION_APPEND_LEMMA2 = prove(
       FIRST_ASSUM(MATCH_MP_TAC o el 3 o
         CONJUNCTS o REWRITE_RULE[DIVISION_THM]) THEN
       REWRITE_TAC[GREATER_EQ, SUB_LEFT_LESS_EQ] THEN
-      ONCE_REWRITE_TAC[ADD_SYM] THEN ASM_REWRITE_TAC[]]]]);
+      ONCE_REWRITE_TAC[ADD_SYM] THEN ASM_REWRITE_TAC[]]]]
+QED
 
-val DIVISION_APPEND = store_thm("DIVISION_APPEND",
-  Term`!a b c.
+(* added ‘g’ into quantifiers *)
+Theorem DIVISION_APPEND :
+   !g a b c.
       (?D1 p1. tdiv(a,b) (D1,p1) /\ fine(g) (D1,p1)) /\
       (?D2 p2. tdiv(b,c) (D2,p2) /\ fine(g) (D2,p2)) ==>
-        ?D p. tdiv(a,c) (D,p) /\ fine(g) (D,p)`,
+        ?D p. tdiv(a,c) (D,p) /\ fine(g) (D,p)
+Proof
   REPEAT STRIP_TAC THEN MAP_EVERY EXISTS_TAC [D_tm, p_tm] THEN
   DISJ_CASES_TAC(GSYM (SPEC (Term`dsize(D1)`) LESS_0_CASES)) THENL
    [ASM_REWRITE_TAC[NOT_LESS_0, SUB_0] THEN
@@ -2793,16 +2843,18 @@ val DIVISION_APPEND = store_thm("DIVISION_APPEND",
     MATCH_MP_TAC LESS_EQUAL_ANTISYM THEN
     ASM_REWRITE_TAC[GSYM NOT_LESS] THEN REWRITE_TAC[NOT_LESS] THEN
     MATCH_MP_TAC LESS_OR THEN ASM_REWRITE_TAC[],
-    ASM_REWRITE_TAC[SUB]]);
+    ASM_REWRITE_TAC[SUB]]
+QED
 
 (* ------------------------------------------------------------------------ *)
 (* We can always find a division which is fine wrt any gauge                *)
 (* ------------------------------------------------------------------------ *)
 
-val DIVISION_EXISTS = store_thm("DIVISION_EXISTS",
- Term `!a b g. a <= b /\ gauge(\x. a <= x /\ x <= b) g
+Theorem DIVISION_EXISTS :
+   !a b g. a <= b /\ gauge(\x. a <= x /\ x <= b) g
                 ==>
-                ?D p. tdiv(a,b) (D,p) /\ fine(g) (D,p)`,
+                ?D p. tdiv(a,b) (D,p) /\ fine(g) (D,p)
+Proof
   REPEAT GEN_TAC THEN DISCH_THEN(CONJUNCTS_THEN2 MP_TAC ASSUME_TAC) THEN
   (MP_TAC o C SPEC BOLZANO_LEMMA)
     (Term `\(u,v). a <= u /\ v <= b
@@ -2855,24 +2907,25 @@ val DIVISION_EXISTS = store_thm("DIVISION_EXISTS",
       ASM_REWRITE_TAC[num_CONV (Term`1:num`), LESS_THM, NOT_LESS_0] THEN
       DISCH_THEN SUBST1_TAC THEN ASM_REWRITE_TAC[],
       DISCH_THEN(SUBST1_TAC o MATCH_MP DIVISION_0) THEN
-      REWRITE_TAC[NOT_LESS_0]]]);
+      REWRITE_TAC[NOT_LESS_0]]]
+QED
 
 (* ------------------------------------------------------------------------ *)
 (* Lemmas about combining gauges                                            *)
 (* ------------------------------------------------------------------------ *)
 
 val GAUGE_MIN = store_thm("GAUGE_MIN",
-  Term`!E g1 g2. gauge(E) g1 /\ gauge(E) g2 ==>
-        gauge(E) (\x. if g1(x) < g2(x) then g1(x) else g2(x))`,
+  ``!E g1 g2. gauge(E) g1 /\ gauge(E) g2 ==>
+        gauge(E) (\x. if g1(x) < g2(x) then g1(x) else g2(x))``,
   REPEAT GEN_TAC THEN REWRITE_TAC[gauge] THEN STRIP_TAC THEN
   X_GEN_TAC (Term`x:real`) THEN BETA_TAC THEN DISCH_TAC THEN
   COND_CASES_TAC THEN FIRST_ASSUM MATCH_MP_TAC THEN
   FIRST_ASSUM ACCEPT_TAC);;
 
 val FINE_MIN = store_thm("FINE_MIN",
-  Term`!g1 g2 D p.
+  ``!g1 g2 D p.
         fine (\x. if g1(x) < g2(x) then g1(x) else g2(x)) (D,p) ==>
-        fine(g1) (D,p) /\ fine(g2) (D,p)`,
+        fine(g1) (D,p) /\ fine(g2) (D,p)``,
   REPEAT GEN_TAC THEN REWRITE_TAC[fine] THEN
   BETA_TAC THEN DISCH_TAC THEN CONJ_TAC THEN
   X_GEN_TAC (Term`n:num`) THEN DISCH_THEN(ANTE_RES_THEN MP_TAC) THEN
@@ -2888,8 +2941,8 @@ val FINE_MIN = store_thm("FINE_MIN",
 (* ------------------------------------------------------------------------ *)
 
 val DINT_UNIQ = store_thm("DINT_UNIQ",
- Term`!a b f k1 k2.
-        a <= b /\ Dint(a,b) f k1 /\ Dint(a,b) f k2 ==> (k1 = k2)`,
+ ``!a b f k1 k2.
+        a <= b /\ Dint(a,b) f k1 /\ Dint(a,b) f k2 ==> (k1 = k2)``,
   REPEAT GEN_TAC THEN DISCH_THEN(CONJUNCTS_THEN2 ASSUME_TAC MP_TAC) THEN
   GEN_REWRITE_TAC RAND_CONV [] [GSYM REAL_SUB_0] THEN
   CONV_TAC CONTRAPOS_CONV THEN ONCE_REWRITE_TAC[ABS_NZ] THEN DISCH_TAC THEN
@@ -2929,15 +2982,17 @@ val DINT_UNIQ = store_thm("DINT_UNIQ",
 (* Integral over a null interval is 0                                       *)
 (* ------------------------------------------------------------------------ *)
 
-val INTEGRAL_NULL = store_thm("INTEGRAL_NULL",
-  Term`!f a. Dint(a,a) f (&0)`,
+Theorem INTEGRAL_NULL :
+   !f a. Dint(a,a) f (&0)
+Proof
   REPEAT GEN_TAC THEN REWRITE_TAC[Dint] THEN GEN_TAC THEN
   DISCH_TAC THEN EXISTS_TAC (Term`\x:real. &1`) THEN
   REWRITE_TAC[gauge, REAL_LT_01] THEN REPEAT GEN_TAC THEN
   REWRITE_TAC[tdiv] THEN STRIP_TAC THEN
   FIRST_ASSUM(MP_TAC o MATCH_MP DIVISION_EQ) THEN
   REWRITE_TAC[rsum] THEN DISCH_THEN SUBST1_TAC THEN
-  ASM_REWRITE_TAC[sum, REAL_SUB_REFL, ABS_0]);;
+  ASM_REWRITE_TAC[sum, REAL_SUB_REFL, ABS_0]
+QED
 
 (* ------------------------------------------------------------------------ *)
 (* Fundamental theorem of calculus (Part I)                                 *)
@@ -3044,7 +3099,7 @@ val STRADDLE_LEMMA = prove(
          (Term`(a * b) * c = (a * c) * b`)] THEN
      REWRITE_TAC[GSYM REAL_MUL_ASSOC,
         MATCH_MP REAL_LE_LMUL (ASSUME (Term`&0 < e`))] THEN
-      SUBGOAL_THEN (Term`!x y. (x * inv(&2)) <= (y * inv(&2)) = x <= y`)
+      SUBGOAL_THEN (Term`!x y. (x * inv(&2)) <= (y * inv(&2)) <=> x <= y`)
       (fn th => ASM_REWRITE_TAC[th, real_sub, REAL_LE_LADD, REAL_LE_NEG]) THEN
       REPEAT GEN_TAC THEN MATCH_MP_TAC REAL_LE_RMUL THEN
       MATCH_MP_TAC REAL_INV_POS THEN
@@ -3065,7 +3120,7 @@ val STRADDLE_LEMMA = prove(
         (Term `(a * b) * c = (a * c) * b`)] THEN
       REWRITE_TAC[GSYM REAL_MUL_ASSOC,
         MATCH_MP REAL_LE_LMUL (ASSUME (Term`&0 < e`))] THEN
-      SUBGOAL_THEN (Term`!x y. (x * inv(&2)) <= (y * inv(&2)) = x <= y`)
+      SUBGOAL_THEN (Term`!x y. (x * inv(&2)) <= (y * inv(&2)) <=> x <= y`)
       (fn th => ASM_REWRITE_TAC[th, real_sub, REAL_LE_RADD, REAL_LE_NEG]) THEN
       REPEAT GEN_TAC THEN MATCH_MP_TAC REAL_LE_RMUL THEN
       MATCH_MP_TAC REAL_INV_POS THEN
@@ -3162,16 +3217,16 @@ val EXT_CONV =  SYM o uncurry X_FUN_EQ_CONV o
 
 val _ = Parse.hide "B";
 
-val MCLAURIN = store_thm("MCLAURIN",
- Term
-  `!f diff h n.
+Theorem MCLAURIN :
+   !f diff h n.
     &0 < h /\ 0 < n /\ (diff(0) = f) /\
     (!m t. m < n /\ &0 <= t /\ t <= h ==>
            (diff(m) diffl diff(SUC m)(t))(t)) ==>
-   (?t. &0 < t /\ t < h /\
+    (?t. &0 < t /\ t < h /\
         (f(h) = sum(0,n)(\m. (diff(m)(&0) / &(FACT m)) * (h pow m))
                 +
-                ((diff(n)(t) / &(FACT n)) * (h pow n))))`,
+                ((diff(n)(t) / &(FACT n)) * (h pow n))))
+Proof
   REPEAT GEN_TAC THEN STRIP_TAC THEN
   UNDISCH_TAC (Term`0 < n:num`) THEN
   DISJ_CASES_THEN2 SUBST_ALL_TAC (X_CHOOSE_THEN (Term`r:num`) MP_TAC)
@@ -3387,7 +3442,8 @@ val MCLAURIN = store_thm("MCLAURIN",
       DISCH_THEN(X_CHOOSE_THEN (Term`t:real`) STRIP_ASSUME_TAC) THEN
       EXISTS_TAC (Term`t:real`) THEN ASM_REWRITE_TAC[] THEN
       MATCH_MP_TAC REAL_LT_TRANS THEN EXISTS_TAC (Term`t0:real`) THEN
-      ASM_REWRITE_TAC[]]]);
+      ASM_REWRITE_TAC[]]]
+QED
 
 Theorem MCLAURIN_NEG:
   !f diff h n.
@@ -3405,7 +3461,7 @@ Proof
   BETA_TAC THEN ASM_REWRITE_TAC[REAL_NEG_GT0, pow, REAL_MUL_LID] THEN
   ONCE_REWRITE_TAC[GSYM REAL_LE_NEG] THEN
   REWRITE_TAC[REAL_NEGNEG, REAL_NEG_0] THEN
-  ONCE_REWRITE_TAC[TAUT_CONV (Term`a /\ b /\ c = a /\ c /\ b`)] THEN
+  ONCE_REWRITE_TAC[TAUT_CONV (Term`a /\ b /\ c <=> a /\ c /\ b`)] THEN
   W(C SUBGOAL_THEN (fn t => REWRITE_TAC[t]) o funpow 2 (fst o dest_imp) o snd)
   THENL
    [REPEAT GEN_TAC THEN
@@ -3438,8 +3494,8 @@ QED
 (* Simple strong form if a function is differentiable everywhere.            *)
 (* ------------------------------------------------------------------------- *)
 
-val MCLAURIN_ALL_LT = store_thm("MCLAURIN_ALL_LT",
- Term`!f diff.
+Theorem MCLAURIN_ALL_LT :
+   !f diff.
       (diff 0 = f) /\
       (!m x. ((diff m) diffl (diff(SUC m) x)) x)
       ==> !x n. ~(x = &0) /\ 0 < n
@@ -3447,7 +3503,8 @@ val MCLAURIN_ALL_LT = store_thm("MCLAURIN_ALL_LT",
                     (f(x) = sum(0,n)
                                 (\m. (diff m (&0) / &(FACT m)) * x pow m)
                             +
-                            (diff n t / &(FACT n)) * x pow n)`,
+                            (diff n t / &(FACT n)) * x pow n)
+Proof
   REPEAT STRIP_TAC THEN
   REPEAT_TCL DISJ_CASES_THEN MP_TAC
    (SPECL [Term`x:real`, Term`&0`] REAL_LT_TOTAL) THEN
@@ -3465,14 +3522,16 @@ val MCLAURIN_ALL_LT = store_thm("MCLAURIN_ALL_LT",
     DISCH_THEN(X_CHOOSE_THEN (Term`t:real`) STRIP_ASSUME_TAC) THEN
     EXISTS_TAC (Term`t:real`) THEN ASM_REWRITE_TAC[] THEN
     UNDISCH_TAC (Term`&0 < t`) THEN UNDISCH_TAC (Term`t < x`)
-    THEN REAL_ARITH_TAC]);
+    THEN REAL_ARITH_TAC]
+QED
 
-val MCLAURIN_ZERO = store_thm("MCLAURIN_ZERO",
- Term`!diff n x. (x = &0) /\ 0 < n
+Theorem MCLAURIN_ZERO :
+   !diff n x. (x = &0) /\ 0 < n
        ==>
        (sum(0,n) (\m. (diff m (&0) / &(FACT m)) * x pow m)
         =
-       diff 0 (&0))`,
+       diff 0 (&0))
+Proof
   REPEAT GEN_TAC THEN DISCH_THEN(CONJUNCTS_THEN2 SUBST1_TAC MP_TAC) THEN
   SPEC_TAC(Term`n:num`,Term`n:num`) THEN INDUCT_TAC THEN
   REWRITE_TAC[LESS_REFL] THEN REWRITE_TAC[LESS_THM] THEN
@@ -3488,29 +3547,34 @@ val MCLAURIN_ZERO = store_thm("MCLAURIN_ZERO",
     UNDISCH_TAC (Term`0 < n:num`) THEN SPEC_TAC(Term`n:num`,Term`n:num`) THEN
     INDUCT_TAC THEN BETA_TAC THEN REWRITE_TAC[LESS_REFL] THEN
     REWRITE_TAC[ADD_CLAUSES, pow, REAL_MUL_LZERO, REAL_MUL_RZERO] THEN
-    REWRITE_TAC[REAL_ADD_RID]]);
+    REWRITE_TAC[REAL_ADD_RID]]
+QED
 
+Theorem LET_CASES[local] :
+   !m n:num. m <= n \/ n < m
+Proof
+  ONCE_REWRITE_TAC [DISJ_SYM] THEN MATCH_ACCEPT_TAC LESS_CASES
+QED
 
-
-val LET_CASES = prove(Term`!m n:num. m <= n \/ n < m`,
-ONCE_REWRITE_TAC [DISJ_SYM] THEN MATCH_ACCEPT_TAC LESS_CASES);
-
-val REAL_POW_EQ_0 = prove
- (Term`!x n. (x pow n = &0) = (x = &0) /\ ~(n = 0)`,
+Theorem REAL_POW_EQ_0[local] :
+   !x n. (x pow n = &0) <=> (x = &0) /\ ~(n = 0)
+Proof
   GEN_TAC THEN INDUCT_TAC THEN
   ASM_REWRITE_TAC[NOT_SUC, pow, REAL_ENTIRE] THENL
    [REWRITE_TAC [REAL_OF_NUM_EQ, ONE,NOT_SUC],
-    EQ_TAC THEN REPEAT STRIP_TAC THEN ASM_REWRITE_TAC[]]);
+    EQ_TAC THEN REPEAT STRIP_TAC THEN ASM_REWRITE_TAC[]]
+QED
 
-val MCLAURIN_ALL_LE = store_thm("MCLAURIN_ALL_LE",
- Term`!f diff.
+Theorem MCLAURIN_ALL_LE :
+   !f diff.
       (diff 0 = f) /\
       (!m x. ((diff m) diffl (diff(SUC m) x)) x)
       ==> !x n. ?t. abs t  <= abs x /\
                    (f(x) = sum(0,n)
                              (\m. (diff m (&0) / &(FACT m)) * x pow m)
                            +
-                            (diff n t / &(FACT n)) * x pow n)`,
+                            (diff n t / &(FACT n)) * x pow n)
+Proof
   REPEAT STRIP_TAC THEN
   DISJ_CASES_THEN MP_TAC(SPECL [Term`n:num`, Term`0:num`] LET_CASES) THENL
    [REWRITE_TAC[LE] THEN DISCH_THEN SUBST1_TAC THEN
@@ -3527,79 +3591,73 @@ val MCLAURIN_ALL_LE = store_thm("MCLAURIN_ALL_LE",
       DISCH_THEN(MP_TAC o SPEC_ALL) THEN ASM_REWRITE_TAC[] THEN
       DISCH_THEN(X_CHOOSE_THEN (Term`t:real`) STRIP_ASSUME_TAC) THEN
       EXISTS_TAC (Term`t:real`) THEN ASM_REWRITE_TAC[] THEN
-      MATCH_MP_TAC REAL_LT_IMP_LE THEN ASM_REWRITE_TAC[]]]);
-
+      MATCH_MP_TAC REAL_LT_IMP_LE THEN ASM_REWRITE_TAC[]]]
+QED
 
 (* ------------------------------------------------------------------------- *)
 (* Version for exp.                                                          *)
 (* ------------------------------------------------------------------------- *)
 
-val MCLAURIN_EXP_LEMMA = prove
- (Term`((\n:num. exp) 0 = exp) /\
-   (!m x. (((\n:num. exp) m) diffl ((\n:num. exp) (SUC m) x)) x)`,
-  REWRITE_TAC[DIFF_EXP]);
+Theorem MCLAURIN_EXP_LEMMA[local] :
+   ((\n:num. exp) 0 = exp) /\
+   (!m x. (((\n:num. exp) m) diffl ((\n:num. exp) (SUC m) x)) x)
+Proof
+  REWRITE_TAC[DIFF_EXP]
+QED
 
-val MCLAURIN_EXP_LT = store_thm("MCLAURIN_EXP_LT",
- Term`!x n. ~(x = &0) /\ 0 < n
+Theorem MCLAURIN_EXP_LT :
+   !x n. ~(x = &0) /\ 0 < n
          ==> ?t. &0 < abs(t) /\
                  abs(t) < abs(x) /\
                  (exp(x) = sum(0,n)(\m. x pow m / &(FACT m)) +
-                           (exp(t) / &(FACT n)) * x pow n)`,
+                           (exp(t) / &(FACT n)) * x pow n)
+Proof
   MP_TAC (MATCH_MP MCLAURIN_ALL_LT MCLAURIN_EXP_LEMMA) THEN BETA_TAC THEN
   REPEAT STRIP_TAC THEN RES_TAC THEN NTAC 3 (POP_ASSUM (K ALL_TAC)) THEN
   EXISTS_TAC (Term`t:real`) THEN
   ASM_REWRITE_TAC [EXP_0,real_div,REAL_MUL_LID,REAL_MUL_RID]
   THEN AP_THM_TAC THEN AP_TERM_TAC THEN AP_TERM_TAC THEN CONV_TAC FUN_EQ_CONV
   THEN GEN_TAC THEN BETA_TAC THEN GEN_REWRITE_TAC LAND_CONV [] [REAL_MUL_SYM]
-  THEN REFL_TAC);
+  THEN REFL_TAC
+QED
 
-val MCLAURIN_EXP_LE = store_thm("MCLAURIN_EXP_LE",
- Term`!x n. ?t. abs(t) <= abs(x) /\
+Theorem MCLAURIN_EXP_LE :
+   !x n. ?t. abs(t) <= abs(x) /\
              (exp(x) = sum(0,n)(\m. x pow m / &(FACT m)) +
-                       (exp(t) / &(FACT n)) * x pow n)`,
+                       (exp(t) / &(FACT n)) * x pow n)
+Proof
   MP_TAC (MATCH_MP MCLAURIN_ALL_LE MCLAURIN_EXP_LEMMA) THEN
   DISCH_THEN (fn th => REPEAT GEN_TAC THEN STRIP_ASSUME_TAC (SPEC_ALL th))
   THEN EXISTS_TAC (Term`t:real`) THEN  ASM_REWRITE_TAC [] THEN
   AP_THM_TAC THEN REPEAT AP_TERM_TAC THEN CONV_TAC FUN_EQ_CONV
   THEN GEN_TAC THEN BETA_TAC THEN
   REWRITE_TAC[EXP_0, real_div, REAL_MUL_LID, REAL_MUL_RID] THEN
-  GEN_REWRITE_TAC LAND_CONV [] [REAL_MUL_SYM] THEN REFL_TAC);
+  GEN_REWRITE_TAC LAND_CONV [] [REAL_MUL_SYM] THEN REFL_TAC
+QED
 
 (* ------------------------------------------------------------------------- *)
 (* Version for ln(1 - x).                                                    *)
 (* ------------------------------------------------------------------------- *)
 
-val DIFF_LN_COMPOSITE = store_thm("DIFF_LN_COMPOSITE",
- Term`!g m x. (g diffl m)(x) /\ &0 < g x
-           ==> ((\x. ln(g x)) diffl (inv(g x) * m))(x)`,
+Theorem DIFF_LN_COMPOSITE :
+   !g m x. (g diffl m)(x) /\ &0 < g x
+           ==> ((\x. ln(g x)) diffl (inv(g x) * m))(x)
+Proof
   REPEAT STRIP_TAC THEN MATCH_MP_TAC DIFF_CHAIN THEN
   ASM_REWRITE_TAC[] THEN MATCH_MP_TAC DIFF_LN THEN
-  ASM_REWRITE_TAC[]);
+  ASM_REWRITE_TAC[]
+QED
 
 val _ = basic_diffs := !basic_diffs@[SPEC_ALL DIFF_LN_COMPOSITE];
 
 val lem = prove(Term`!n:num. 0 < n ==> ~(n=0)`,
 INDUCT_TAC THEN ASM_REWRITE_TAC [NOT_SUC,NOT_LESS_0]);
 
-(* ----------------------------------------------------------------------
-    Exponentiation with real exponents
-
-    Contributed by
-
-       Umair Siddique
-
-       Email: umair.siddique@rcms.nust.edu.pk
-       DATE: 29-12-2010
-
-       System Analysis & Verification (sAvE)  LAB
-
-       National University of Sciences and Technology (NUST)
-       Ialamabad,Pakistan
-    ---------------------------------------------------------------------- *)
+(* ------------------------------------------------------------------------- *)
+(* Exponentiation with real exponents (rpow)                                 *)
+(* ------------------------------------------------------------------------- *)
 
 fun K_TAC _ = ALL_TAC;
-
-open bossLib realSimps
 
 (* Definition *)
 val _ = set_fixity "rpow" (Infixr 700);
@@ -3710,17 +3768,16 @@ val  RPOW_RPOW= store_thm
   RW_TAC real_ss [rpow, LN_EXP, REAL_MUL_ASSOC] THEN
   PROVE_TAC[ REAL_MUL_COMM] );
 
-
-val  RPOW_LT= store_thm
-        ("RPOW_LT",
-        ``! (a:real) (b:real) (c:real).(1 < a)==>((a rpow b < a rpow c)= b < c )``,
+Theorem RPOW_LT :
+   !(a:real) (b:real) (c:real). 1 < a ==> (a rpow b < a rpow c <=> b < c)
+Proof
  RW_TAC std_ss [rpow]  THEN
- KNOW_TAC`` exp (b * ln a) < exp (c * ln a)= (b*ln a < c*ln a)``  THEN1
+ KNOW_TAC`` exp (b * ln a) < exp (c * ln a) <=> (b*ln a < c*ln a)``  THEN1
       RW_TAC real_ss [EXP_MONO_LT]  THEN
       DISCH_TAC THEN ASM_REWRITE_TAC[] THEN POP_ASSUM K_TAC  THEN
-      KNOW_TAC``((b:real)*ln a < (c:real)*ln a)= (b < c)``  THENL   [
+      KNOW_TAC``((b:real)*ln a < (c:real)*ln a) <=> (b < c)``  THENL   [
       MATCH_MP_TAC REAL_LT_RMUL  THEN
-      KNOW_TAC``0 < ln a = exp (0) < exp (ln a)``  THEN1
+      KNOW_TAC``0 < ln a <=> exp (0) < exp (ln a)``  THEN1
          PROVE_TAC[EXP_MONO_LT]  THEN
          DISCH_TAC  THEN
          FULL_SIMP_TAC real_ss[]  THEN
@@ -3734,18 +3791,20 @@ val  RPOW_LT= store_thm
              KNOW_TAC``exp (ln a)=(a:real)``  THEN1
                   RW_TAC real_ss [EXP_LN] THEN
                   DISCH_TAC THEN ASM_REWRITE_TAC[]],
-            RW_TAC real_ss []]);
+            RW_TAC real_ss []]
+QED
 
-val  RPOW_LE = store_thm
-        ("RPOW_LE",
-        ``!a b c. (1 < a)==>((a rpow b <= a rpow c)= b <= c )``,
+Theorem RPOW_LE :
+   !a b c. 1 < a ==> (a rpow b <= a rpow c <=> b <= c)
+Proof
  RW_TAC std_ss [rpow] THEN
- KNOW_TAC`` exp ((b:real) * ln a) <= exp ((c:real) * ln a)= ((b:real)*ln a <= (c:real)*ln a)`` THEN1
+ KNOW_TAC ``exp ((b:real) * ln a) <= exp ((c:real) * ln a) <=>
+            ((b:real)*ln a <= (c:real)*ln a)`` THEN1
       RW_TAC real_ss [EXP_MONO_LE] THEN
  DISCH_TAC THEN ASM_REWRITE_TAC[] THEN POP_ASSUM K_TAC THEN
- KNOW_TAC``(b*ln a <= c*ln a)= ((b:real) <= (c:real))`` THENL[
+ KNOW_TAC``(b*ln a <= c*ln a) <=> ((b:real) <= (c:real))`` THENL[
           MATCH_MP_TAC REAL_LE_RMUL THEN
-     KNOW_TAC``0 < ln a = exp (0) < exp (ln a)`` THEN1
+     KNOW_TAC``0 < ln a <=> exp (0) < exp (ln a)`` THEN1
          PROVE_TAC[EXP_MONO_LT] THEN
           DISCH_TAC THEN
           FULL_SIMP_TAC real_ss[] THEN
@@ -3759,60 +3818,60 @@ val  RPOW_LE = store_thm
           KNOW_TAC``exp (ln a)=(a:real)`` THEN1
              RW_TAC real_ss [EXP_LN] THEN
              DISCH_TAC THEN ASM_REWRITE_TAC[]],
- RW_TAC real_ss []]);
+ RW_TAC real_ss []]
+QED
 
-
-val  BASE_RPOW_LE= store_thm
-        ("BASE_RPOW_LE",
-        ``! a b c. (0 < a)/\ (0 < c)/\ (0 < b)==>((a rpow b <= c rpow b)= a <= c )``,
+Theorem BASE_RPOW_LE :
+   !a b c. 0 < a /\ 0 < c /\ 0 < b ==> (a rpow b <= c rpow b <=> a <= c)
+Proof
 RW_TAC std_ss [rpow, EXP_MONO_LE] THEN
-KNOW_TAC`` (((b:real) * ln a) <= ((b:real) * ln c))= ((ln a <= ln c))`` THENL[
+KNOW_TAC`` (((b:real) * ln a) <= ((b:real) * ln c)) <=> ((ln a <= ln c))`` THENL[
   MATCH_MP_TAC REAL_LE_LMUL   THEN
   RW_TAC real_ss [],
 
   DISCH_TAC THEN ASM_REWRITE_TAC[] THEN POP_ASSUM K_TAC  THEN
-  RW_TAC real_ss [LN_MONO_LE]]);
+  RW_TAC real_ss [LN_MONO_LE]]
+QED
 
-val  BASE_RPOW_LT= store_thm
-        ("BASE_RPOW_LT",
-        ``! a b c. (0 < a)/\ (0 < c)/\ (0 < b)==>((a rpow b < c rpow b)= a < c )``,
-
+Theorem BASE_RPOW_LT :
+   !a b c. 0 < a /\ 0 < c /\ 0 < b ==> (a rpow b < c rpow b <=> a < c)
+Proof
  RW_TAC std_ss [rpow, EXP_MONO_LT]  THEN
- KNOW_TAC ``((b * ln a) < (b * ln c))= ((ln a < ln c))``  THENL[
+ KNOW_TAC ``((b * ln a) < (b * ln c)) <=> ln a < ln c``  THENL[
        MATCH_MP_TAC REAL_LT_LMUL  THEN
-       RW_TAC real_ss []  ,
+       RW_TAC real_ss [],
 
        DISCH_TAC THEN ASM_REWRITE_TAC[] THEN POP_ASSUM K_TAC  THEN
-       RW_TAC real_ss [LN_MONO_LT] ]);
+       RW_TAC real_ss [LN_MONO_LT] ]
+QED
 
-val  RPOW_UNIQ_BASE= store_thm (
-  "RPOW_UNIQ_BASE",
-  ``!a b c. 0 < a /\ 0 < c /\ 0 <> b /\ (a rpow b = c rpow b)==> (a = c)``,
-
-
- RW_TAC std_ss [rpow, GSYM LN_INJ]THEN
+Theorem RPOW_UNIQ_BASE :
+   !a b c. 0 < a /\ 0 < c /\ 0 <> b /\ (a rpow b = c rpow b) ==> (a = c)
+Proof
+ RW_TAC std_ss [rpow, GSYM LN_INJ] THEN
  POP_ASSUM MP_TAC  THEN
- KNOW_TAC`` (exp (b * ln a) = exp (b * ln c)) = (ln (exp (b * ln a)) = ln (exp (b * ln c)))``THEN1
+ KNOW_TAC ``(exp (b * ln a) = exp (b * ln c)) <=>
+            (ln (exp (b * ln a)) = ln (exp (b * ln c)))``THEN1
      PROVE_TAC[LN_EXP]THEN
      DISCH_TAC THEN ASM_REWRITE_TAC[] THEN POP_ASSUM K_TAC THEN
      FULL_SIMP_TAC real_ss[LN_EXP] THEN
-     FULL_SIMP_TAC real_ss[REAL_EQ_MUL_LCANCEL]);
+     FULL_SIMP_TAC real_ss[REAL_EQ_MUL_LCANCEL]
+QED
 
-
-val  RPOW_UNIQ_EXP = store_thm
-        ("RPOW_UNIQ_EXP",
-        ``!a b c. 1 < a /\ 0 < c /\ 0 < b /\ (a rpow b = a rpow c) ==>
-                  (b = c)``,
+Theorem RPOW_UNIQ_EXP :
+   !a b c. 1 < a /\ 0 < c /\ 0 < b /\ (a rpow b = a rpow c) ==> (b = c)
+Proof
  RW_TAC std_ss [rpow, GSYM LN_INJ] THEN
  POP_ASSUM MP_TAC THEN
- KNOW_TAC`` (exp (b * ln a) = exp (c * ln a)) = (ln (exp (b * ln a)) = ln (exp (c * ln a)))`` THEN1
+ KNOW_TAC ``(exp (b * ln a) = exp (c * ln a)) <=>
+            (ln (exp (b * ln a)) = ln (exp (c * ln a)))`` THEN1
       PROVE_TAC[LN_EXP] THEN
           DISCH_TAC THEN ASM_REWRITE_TAC[] THEN POP_ASSUM K_TAC THEN
           FULL_SIMP_TAC real_ss[LN_EXP] THEN
           FULL_SIMP_TAC real_ss[REAL_EQ_RMUL] THEN
           KNOW_TAC``(1 < (a:real))==> 0 < ln a`` THENL[
       RW_TAC real_ss [] THEN
-      KNOW_TAC``0 < ln a = exp (0) < exp (ln a)`` THEN1
+      KNOW_TAC``0 < ln a <=> exp (0) < exp (ln a)`` THEN1
           PROVE_TAC[EXP_MONO_LT] THEN
           DISCH_TAC THEN
           FULL_SIMP_TAC real_ss[] THEN
@@ -3826,15 +3885,17 @@ val  RPOW_UNIQ_EXP = store_thm
                    KNOW_TAC``exp (ln a)=(a:real)`` THEN1
                       RW_TAC real_ss [EXP_LN] THEN
        DISCH_TAC THEN ASM_REWRITE_TAC[] THEN  RW_TAC real_ss []],
- FULL_SIMP_TAC real_ss[REAL_POS_NZ] ]);
+ FULL_SIMP_TAC real_ss[REAL_POS_NZ] ]
+QED
 
-val  RPOW_DIV_BASE= store_thm
-        ("RPOW_DIV_BASE",
-        `` ! x t. (0 < x)==> ((x rpow t)/x = x rpow (t-1))``,
+Theorem RPOW_DIV_BASE :
+   !x t. 0 < x ==> ((x rpow t)/x = x rpow (t-1))
+Proof
 RW_TAC std_ss [rpow, REAL_SUB_RDISTRIB, EXP_SUB, REAL_MUL_LID] THEN
 KNOW_TAC``exp(ln x)= (x:real)`` THEN1
     PROVE_TAC[EXP_LN] THEN
-DISCH_TAC THEN ASM_REWRITE_TAC [] );
+DISCH_TAC THEN ASM_REWRITE_TAC []
+QED
 
 (*----------------------------------------------------------------*)
 (* Differentiability of real powers                               *)
